fixed per-component config, init_msg, and other details

compiler/dsl/ml/primitives/Main.ml
@@ -1,1 +1,2 @@
-STImpl.exec (ReflexSSH.main) ()
+(* Please leave Echo here on the repo, feel free to change it locally, don't push *)
+STImpl.exec (ReflexEcho.main) ()
