compiler/dsl/coq/Reflex.v
@@ -1,4 +1,5 @@
 Require Import Ascii.
+Require Import Bool.
 Require Import Eqdep_dec.
 Require Import NPeano.
 Require Import List.
@@ -87,14 +88,18 @@ Section WITH_PAYLOAD_DESC_VEC.
 Context {NB_MSG : nat}.
 Variable VVD : vvdesc NB_MSG.
 
-(* might as well put this here *)
-Variable COMPT : Type.
-Record comp :=
-{ comp_name : str
-; comp_cmd  : str
-; comp_args : list str
+Record compd :=
+{ compd_name : str
+; compd_cmd  : str
+; compd_args : list str
+; compd_conf : vdesc
 }.
-Variable COMPS : COMPT -> comp.
+
+Variable COMPT : Set.
+
+Variable COMPTDEC : forall (x y : COMPT), decide (x = y).
+
+Variable COMPS : COMPT -> compd.
 
 Definition lkup_tag (tag : fin NB_MSG) : vdesc :=
   vec_ith VVD tag.
@@ -420,13 +425,66 @@ Variable KSTD : vdesc.
 Notation KSTD_SIZE := (projT1 KSTD).
 Notation KSTD_DESC := (projT2 KSTD).
 
-Context {NB_COMPD:nat}.
-Variable VVD_COMPS : vvdesc NB_COMPD.
+Definition comp_conf_desc compt := compd_conf (COMPS compt).
 
-Definition component := (fd * sigT(fun tag => s[[vec_ith VVD_COMPS tag]]))%type.
+Record comp : Set :=
+{ comp_type : COMPT
+; comp_fd   : fd
+; comp_conf : s[[ comp_conf_desc comp_type ]]
+}.
+
+Definition sdenote_desc_cfg_pat (d:desc) : Set := option (sdenote_desc d).
+
+Record comp_pat : Set :=
+{ comp_pat_type : COMPT
+; comp_pat_fd   : option fd
+; comp_pat_conf : shvec sdenote_desc_cfg_pat (projT2 (comp_conf_desc comp_pat_type))
+}.
+
+Definition elt_match (d:desc) (elt:s[[d]]) (elt':sdenote_desc_cfg_pat d) : bool :=
+  match elt' with
+  | None   => true
+  | Some x =>
+    match d as _d return s[[_d]] -> s[[_d]] -> bool with
+    | num_d => fun elt x => if num_eq x elt then true else false
+    | str_d => fun elt x => if str_eq x elt then true else false
+    | fd_d  => fun elt x => if fd_eq x elt then true else false
+    end elt x
+  end.
+
+Definition match_comp (cp : comp_pat) (c : comp) : bool :=
+  match c, cp with
+  | Build_comp t f cfg, Build_comp_pat t' fp cfgp =>
+    match COMPTDEC t t' with
+    | left EQ =>
+      match fp with None => true | Some f' => if fd_eq f f' then true else false end
+      &&
+      match EQ in _ = _t return
+        shvec sdenote_desc_cfg_pat (projT2 (comp_conf_desc _t)) -> bool
+      with
+      | Logic.eq_refl => fun cfgp =>
+        shvec_match (projT2 (comp_conf_desc t))
+                    sdenote_desc sdenote_desc_cfg_pat
+                    elt_match cfg cfgp
+      end cfgp
+    | right _ => false
+    end
+  end.
+
+Definition find_comp (cp : comp_pat) (comps : list comp) :=
+  find (match_comp cp) comps.
+
+Definition filter_comps (cp : comp_pat) (comps : list comp) :=
+  filter (match_comp cp) comps.
+
+Definition exists_comp (cp : comp_pat) (comps : list comp) :=
+  match find_comp cp comps with
+  | None   => false
+  | Some _ => true
+  end.
 
 Record kstate : Set := mkst
-  { kcs : list component
+  { kcs : list comp
   ; ktr : [KTrace]
   ; kst : s[[ KSTD ]]
   ; kfd : list fd (* need to keep track of all the open fds... *)
@@ -572,8 +630,8 @@ Definition env_fds_in l (envd : vdesc) (env : s[[ envd ]]) : Prop :=
   | _ => fun _ => True
   end (shvec_ith _ (projT2 envd) env i).
 
-Definition proj_fds (comps:list component) : list fd :=
-  map (fun comp => match comp with (f, _ ) => f end) comps.
+Definition proj_fds : list comp -> list fd :=
+  map (fun comp => comp_fd comp).
 
 Definition msg_fds_ok : Prop :=
   forall i,
@@ -660,8 +718,9 @@ Definition eval_payload_expr (pd : vdesc) (e : payload_expr pd) : s[[ pd ]] :=
 
 Inductive cmd : Type :=
 | Send  : expr fd_d -> forall (t : fin NB_MSG), payload_expr (lkup_tag t) -> cmd
-| Spawn : COMPT -> forall tag, s[[vec_ith VVD_COMPS tag]] ->
-            forall (i : fin ENVD_SIZE), svec_ith ENVD_DESC i = fd_d -> cmd
+| Spawn :
+    forall (t : COMPT), s[[ comp_conf_desc t ]] ->
+    forall (i : fin ENVD_SIZE), svec_ith ENVD_DESC i = fd_d -> cmd
 | StUpd : forall i, svec_ith (projT2 KSTD) i <> fd_d -> expr (svec_ith (projT2 KSTD) i) -> cmd
 .
 
@@ -761,10 +820,8 @@ Inductive cmd : Type :=
 
 *)
 
-
-
 Record init_state :=
-{ init_comps : list component
+{ init_comps : list comp
 ; init_ktr   : [KTrace]%type
 ; init_env   : s[[ ENVD ]]
 ; init_kst   : s[[ KSTD ]]
@@ -783,7 +840,7 @@ End WITH_PROG_ENV.
 Definition cmd_input_desc (c : cmd)  :=
   match c with
   | Send _ _ _  => None
-  | Spawn _ _ _ _ _ => Some fd_d
+  | Spawn _ _ _ _ => Some fd_d
   | StUpd _ _ _ => None
   end.
 
@@ -814,10 +871,10 @@ Definition init_state_run_cmd (s : init_state) (cmd : cmd) : cmd_input cmd -> in
      ; init_kst   := st
      |}
 
-  | Spawn ct tag cfg i EQ => fun (c:fd) =>
+  | Spawn ct cfg i EQ => fun (c:fd) =>
     let comp := COMPS ct in
-    {| init_comps := (c, existT _ tag cfg) :: cs
-     ; init_ktr   := tr ~~~ KExec (comp_cmd comp) (comp_args comp) c :: tr
+    {| init_comps := {| comp_type := ct; comp_fd := c; comp_conf := cfg |} :: cs
+     ; init_ktr   := tr ~~~ KExec (compd_cmd comp) (compd_args comp) c :: tr
      ; init_env   := shvec_replace_cast EQ e c
      ; init_kst   := st
      |}
@@ -874,11 +931,11 @@ Definition hdlr_state_run_cmd (s : hdlr_state) (cmd : cmd) : cmd_input cmd -> hd
      ; hdlr_env := env
     |}
 
-  | Spawn ct tag cfg i EQ => fun c =>
+  | Spawn ct cfg i EQ => fun c =>
     let comp := COMPS ct in
     {| hdlr_kst :=
-         {| kcs := (c, existT _ tag cfg) :: cs
-          ; ktr := tr ~~~ KExec (comp_cmd comp) (comp_args comp) c :: tr
+         {| kcs := {| comp_type := ct; comp_fd := c; comp_conf := cfg |} :: cs
+          ; ktr := tr ~~~ KExec (compd_cmd comp) (compd_args comp) c :: tr
           ; kst := st
           ; kfd := fd
           |}
@@ -961,14 +1018,13 @@ Variable IENVD : vdesc.
   Problem is with only one language, the MVar expression wants to see a current message,
   but we don't have any in the initial program (in fact, if the user sets NB_MSG := 0,
   messages don't even exist.
-  So for now, we're cheating with init_msg. If the user writes an MVar expression in the
-  initial program, it will raise an exception.
+  So for now, we're cheating with init_msg.
   Eventually, this will be fixed by having a different, reduced language for the initial
   program. Future work as they say! :)
 *)
-Axiom init_msg : msg.
+Variable IMSG : msg.
 
-Variable IPROG : init_prog init_msg IENVD.
+Variable IPROG : init_prog IMSG IENVD.
 
 Definition initial_init_state :=
   {| init_comps := nil
@@ -1006,7 +1062,7 @@ Definition payload_fds (v : vdesc) : s[[ v ]] -> list fd :=
 Inductive Reach : kstate -> Prop :=
 | Reach_init :
   forall s input,
-  s = init_state_run_prog devnull init_msg IENVD initial_init_state IPROG input ->
+  s = init_state_run_prog devnull IMSG IENVD initial_init_state IPROG input ->
   Reach {| kcs := init_comps _ s
          ; ktr := init_ktr _ s
          ; kst := init_kst _ s
@@ -1294,16 +1350,16 @@ Proof.
                  ; init_kst   := st
                  |} }}
 
-    | Spawn ct tag cfg i EQ =>
-      let c_cmd := comp_cmd (COMPS ct) in
-      let c_args := comp_args (COMPS ct) in
+    | Spawn ct cfg i EQ =>
+      let c_cmd := compd_cmd (COMPS ct) in
+      let c_args := compd_args (COMPS ct) in
       c <- exec c_cmd c_args (tr ~~~ expand_ktrace tr)
         <@> open devnull * all_open (proj_fds (init_comps prog_envd s))
           * all_open_payload (init_env prog_envd s)
           * all_open_payload (init_kst prog_envd s);
 
       let tr := tr ~~~ KExec c_cmd c_args c :: tr in
-      {{ Return {| init_comps := (c, existT _ tag cfg) :: cs
+      {{ Return {| init_comps := {| comp_type := ct; comp_fd := c; comp_conf := cfg |} :: cs
                  ; init_ktr   := tr
                  ; init_env   := shvec_replace_cast _ EQ e c
                  ; init_kst   := st
@@ -1614,7 +1670,7 @@ Proof.
 Qed.
 
 Definition run_init_prog :
-  forall (envd : vdesc) (s : init_state envd) (p : init_prog init_msg envd),
+  forall (envd : vdesc) (s : init_state envd) (p : init_prog IMSG envd),
   STsep (tr :~~ init_ktr envd s in
           init_invariant s * traced (expand_ktrace tr))
         (fun s' : init_state envd => tr :~~ init_ktr envd s' in
@@ -1758,15 +1814,15 @@ Proof.
               |}
     }}
 
-  | Spawn ct tag cfg i EQ =>
-    let c_cmd := comp_cmd (COMPS ct) in
-    let c_args := comp_args (COMPS ct) in
+  | Spawn ct cfg i EQ =>
+    let c_cmd := compd_cmd (COMPS ct) in
+    let c_args := compd_args (COMPS ct) in
     c <- exec c_cmd c_args (tr ~~~ expand_ktrace tr)
       <@> all_open ((proj_fds cs) ++ fds) * all_open_payload (pay cm)
         * [In cfd (proj_fds cs)] * [msg_fds_ok st cm] * [env_fds_ok envd s];
 
     let tr := tr ~~~ KExec c_cmd c_args c :: tr in
-    {{ Return {| hdlr_kst := {| kcs := (c, existT _ tag cfg) :: cs
+    {{ Return {| hdlr_kst := {| kcs := {| comp_type := ct; comp_fd := c; comp_conf := cfg |} :: cs
                               ; ktr := tr
                               ; kst := kst st
                               ; kfd := fds |}
@@ -2016,74 +2072,3 @@ Qed.
 End WITH_HANDLER.
 
 End WITH_PAYLOAD_DESC_VEC.
-
-Definition shvec_match_vvdesc {NB_VD:nat}
-  (VVD:vvdesc NB_VD) (tag:fin NB_VD) (tag':fin NB_VD) (sdenote_desc':desc->Set)
-  (elt_match:forall (d:desc), s[[d]] -> sdenote_desc' d -> bool)
-  (v:shvec sdenote_desc (projT2 (lkup_tag VVD tag)))
-  (v':shvec sdenote_desc' (projT2 (lkup_tag VVD tag'))) : bool :=
-  match fin_eq_dec tag tag' with
-  | left H => match H in _ = _tag return
-                shvec sdenote_desc' (projT2 (lkup_tag VVD _tag)) -> bool
-              with
-              | Logic.eq_refl => fun v' =>
-                 shvec_match (projT2 (lkup_tag VVD tag))
-                              sdenote_desc sdenote_desc'
-                              elt_match v v'
-              end v'
-  | right H => false
-  end.
-
-Definition sdenote_desc_cfg_pat (d:desc) :=
-  option (sdenote_desc d).
-
-Definition elt_match
-  (d:desc) (elt:s[[d]]) (elt':sdenote_desc_cfg_pat d) : bool :=
-  match elt' with
-  | None   => true
-  | Some x => match d as _d return
-              s[[_d]] -> s[[_d]] -> bool
-              with
-              | num_d => fun elt x =>
-                           if num_eq x elt then true else false
-              | str_d => fun elt x =>
-                           if str_eq x elt then true else false
-              | fd_d  => fun elt x =>
-                           if fd_eq x elt then true else false
-              end elt x
-  end.
-
-Definition match_comp {NB_CFGD:nat}
-  (optf:option fd) (CFGD:vvdesc NB_CFGD) tag
-  (cfg_pat:shvec sdenote_desc_cfg_pat (projT2 (lkup_tag CFGD tag)))
-  (c:component CFGD) :=
-  match c with
-  | (f',cfg) =>
-    if match optf with
-       | None => true
-       | Some f => if fd_eq f f' then true else false
-       end
-    then shvec_match_vvdesc CFGD _ _ _ elt_match (projT2 cfg) cfg_pat
-    else false
-  end.
-
-Definition find_comp {NB_CFGD:nat}
-  (optf:option fd) (CFGD:vvdesc NB_CFGD) tag
-  (cfg_pat:shvec sdenote_desc_cfg_pat (projT2 (lkup_tag CFGD tag)))
-  (comps:list (component CFGD)) :=
-  find (match_comp optf CFGD tag cfg_pat) comps.
-
-Definition filter_comps {NB_CFGD:nat}
-  (CFGD:vvdesc NB_CFGD) tag
-  (cfg_pat:shvec sdenote_desc_cfg_pat (projT2 (lkup_tag CFGD tag)))
-  (comps:list (component CFGD)) :=
-  filter (match_comp None CFGD tag cfg_pat) comps.
-
-Definition exists_comp {NB_CFGD:nat}
-  (optf:option fd) (CFGD:vvdesc NB_CFGD) tag
-  (cfg_pat:shvec sdenote_desc_cfg_pat (projT2 (lkup_tag CFGD tag)))
-  (comps:list (component CFGD)) :=
-  match find_comp optf CFGD tag cfg_pat comps with
-  | None   => false
-  | Some _ => true
-  end.
