compiler/dsl/coq/ReflexEcho.v
@@ -15,6 +15,8 @@ Definition PAYD : vvdesc NB_MSG := mk_vvdesc
   [ ("M", [str_d])
   ].
 
+Notation "'M'" := (None) (only parsing).
+
 Definition KSTD : vdesc := mk_vdesc [].
 
 Definition IENVD : vdesc := mk_vdesc
@@ -23,30 +25,26 @@ Definition IENVD : vdesc := mk_vdesc
 
 Inductive COMPT : Type := Echo.
 
-Definition COMPS (t : COMPT) : comp :=
+Definition COMPTDEC : forall (x y : COMPT), decide (x = y).
+Proof. decide equality. Defined.
+
+Definition COMPS (t : COMPT) : compd :=
   match t with
-  | Echo => mk_comp "Echo" "test/echo-00/test.py" []
+  | Echo => mk_compd "Echo" "test/echo-00/test.py" [] (mk_vdesc [])
   end.
 
-Definition NB_CFGD := 1.
+Definition IMSG : msg PAYD := @Build_msg _ PAYD M (str_of_string "", tt).
 
-Definition CFGD := mk_vvdesc
-  [("Echo", [str_d])
+Definition INIT : init_prog PAYD COMPT COMPS KSTD IMSG IENVD :=
+  [fun s => Spawn _ _ COMPS _ _ IENVD Echo tt None (Logic.eq_refl _)
   ].
 
-Notation t_cfg_echo := (None) (only parsing).
-
-Definition INIT : init_prog PAYD COMPT KSTD CFGD (init_msg PAYD) IENVD :=
-  [fun s => Spawn _ _ _ CFGD _ IENVD Echo t_cfg_echo
-                  (str_of_string "Echo",tt) None (Logic.eq_refl _)
-  ].
-
-Definition HANDLERS : handlers PAYD COMPT KSTD CFGD :=
+Definition HANDLERS : handlers PAYD COMPT COMPS KSTD :=
   fun (m : msg PAYD) cfd =>
     match m as _m return forall (EQ : _m = m), _ with
     | Build_msg None p => fun EQ =>
       let envd := existT _ 0 tt in
-      existT (fun d => hdlr_prog PAYD COMPT KSTD CFGD _ d) envd (
+      existT (fun d => hdlr_prog PAYD COMPT COMPS KSTD _ d) envd (
         let (msg, _) := p in fun st0 =>
         [ fun s => Send _ _ _ _ _ _ (CFd PAYD _ _ _) None (mvar EQ None, tt) ]
       )
@@ -54,4 +52,4 @@ Definition HANDLERS : handlers PAYD COMPT KSTD CFGD :=
       match bad with end
     end (Logic.eq_refl m).
 
-Definition main := mk_main (Build_spec NB_MSG PAYD IENVD KSTD COMPT COMPS NB_CFGD CFGD INIT HANDLERS).
+Definition main := mk_main (Build_spec NB_MSG PAYD IENVD KSTD COMPT COMPTDEC COMPS IMSG INIT HANDLERS).
